BertognaResponseTimeEDFComp.v
@@ -1,0 +1,377 @@
+Require Import Vbase ScheduleDefs BertognaResponseTimeDefs divround helper
+               ssreflect ssrbool eqtype ssrnat seq fintype bigop div path tuple.
+
+Module ResponseTimeIterationEDF.
+
+  Import Schedule ResponseTimeAnalysis.
+
+  Section Analysis.
+    
+    Context {sporadic_task: eqType}.
+    Variable task_cost: sporadic_task -> nat.
+    Variable task_period: sporadic_task -> nat.
+    Variable task_deadline: sporadic_task -> nat.
+    
+    Let task_with_response_time := (sporadic_task * nat)%type.
+    
+    Context {Job: eqType}.
+    Variable job_cost: Job -> nat.
+    Variable job_deadline: Job -> nat.
+    Variable job_task: Job -> sporadic_task.
+
+    Variable num_cpus: nat.
+
+    (* Next we define the fixed-point iteration for computing
+       Bertogna's response-time bound for any task in ts. *)
+    
+    (*Computation of EDF on list of pairs (T,R)*)
+    
+    Let max_steps (ts: taskset_of sporadic_task) :=
+      \max_(tsk <- ts) task_deadline tsk.
+
+    Let response_time_bound (tsk: sporadic_task) (rt_bounds: seq task_with_response_time)
+                            (delta: time) :=
+      task_cost tsk +
+      div_floor
+       (total_interference_bound_jlfp task_cost task_period tsk rt_bounds delta)
+       num_cpus.
+    
+    Let initial_state (ts: taskset_of sporadic_task) :=
+      map (fun t => (t, task_cost t)) ts.
+    
+    Definition edf_rta_iteration (rt_bounds: seq task_with_response_time) :=
+      map (fun pair : task_with_response_time =>
+             let (tsk, R) := pair in
+               (tsk, response_time_bound tsk rt_bounds R))
+          rt_bounds.
+
+    Definition R_le_deadline (pair: task_with_response_time) :=
+      let (tsk, R) := pair in
+        R <= task_deadline tsk.
+    
+    Definition R_list_edf (ts: taskset_of sporadic_task) :=
+      let R_values := iter (max_steps ts) edf_rta_iteration (initial_state ts) in
+        if (all R_le_deadline R_values) then
+          Some R_values
+        else None.
+    
+    (* The schedulability test simply checks if we got a list of
+       response-time bounds (i.e., if the computation did not fail). *)
+    Definition edf_schedulable (ts: taskset_of sporadic_task) :=
+      R_list_edf ts != None.
+    
+    Section AuxiliaryLemmas.
+
+    End AuxiliaryLemmas.
+    
+    Section Proof.
+
+      (* Consider a task set ts. *)
+      Variable ts: taskset_of sporadic_task.
+      
+      (* Assume the task set has no duplicates, ... *)
+      Hypothesis H_ts_is_a_set: uniq ts.
+
+      (* ...all tasks have valid parameters, ... *)
+      Hypothesis H_valid_task_parameters:
+        valid_sporadic_taskset task_cost task_period task_deadline ts.
+
+      (* ...restricted deadlines, ...*)
+      Hypothesis H_restricted_deadlines:
+        forall tsk, tsk \in ts -> task_deadline tsk <= task_period tsk.
+
+      (* ...and tasks are ordered by increasing priorities. *)
+      (*Hypothesis H_sorted_ts: sorted EDF ts.*)
+
+      (* Next, consider any arrival sequence such that...*)
+      Context {arr_seq: arrival_sequence Job}.
+
+     (* ...all jobs come from task set ts, ...*)
+      Hypothesis H_all_jobs_from_taskset:
+        forall (j: JobIn arr_seq), job_task j \in ts.
+      
+      (* ...they have valid parameters,...*)
+      Hypothesis H_valid_job_parameters:
+        forall (j: JobIn arr_seq),
+          valid_sporadic_job task_cost task_deadline job_cost job_deadline job_task j.
+      
+      (* ... and satisfy the sporadic task model.*)
+      Hypothesis H_sporadic_tasks:
+        sporadic_task_model task_period arr_seq job_task.
+      
+      (* Then, consider any platform with at least one CPU and unit
+         unit execution rate, where...*)
+      Variable rate: Job -> processor num_cpus -> nat.
+      Variable sched: schedule num_cpus arr_seq.
+      Hypothesis H_at_least_one_cpu :
+        num_cpus > 0.
+      Hypothesis H_rate_equals_one :
+        forall j cpu, rate j cpu = 1.
+
+      (* ...jobs only execute after they arrived and no longer
+         than their execution costs,... *)
+      Hypothesis H_jobs_must_arrive_to_execute:
+        jobs_must_arrive_to_execute sched.
+      Hypothesis H_completed_jobs_dont_execute:
+        completed_jobs_dont_execute job_cost rate sched.
+
+      (* ...and do not execute in parallel. *)
+      Hypothesis H_no_parallelism:
+        jobs_dont_execute_in_parallel sched.
+
+      (* Assume the platform satisfies the global scheduling invariant. *)
+      Hypothesis H_global_scheduling_invariant:
+        forall (tsk: sporadic_task) (j: JobIn arr_seq) (t: time),
+          tsk \in ts ->
+          job_task j = tsk ->
+          backlogged job_cost rate sched j t ->
+          count
+            (fun tsk_other : _ =>
+               is_interfering_task_jlfp tsk tsk_other &&
+               task_is_scheduled job_task sched tsk_other t) ts = num_cpus.
+
+      Definition no_deadline_missed_by_task (tsk: sporadic_task) :=
+        task_misses_no_deadline job_cost job_deadline job_task rate sched tsk.
+      Definition no_deadline_missed_by_job :=
+        job_misses_no_deadline job_cost job_deadline rate sched.
+
+      Section HelperLemma.
+        
+        (* The following lemma states that the response-time bounds
+           computed using R_list are valid. *)
+        Lemma R_list_has_response_time_bounds :
+          forall rt_bounds tsk R,
+            R_list_edf ts = Some rt_bounds ->
+            (tsk, R) \in rt_bounds ->
+            forall j : JobIn arr_seq,
+              job_task j = tsk ->
+              completed job_cost rate sched j (job_arrival j + R).
+        Proof.
+          rename H_valid_job_parameters into JOBPARAMS,
+                 H_valid_task_parameters into TASKPARAMS,
+                 H_restricted_deadlines into RESTR,
+                 H_completed_jobs_dont_execute into COMP,
+                 H_jobs_must_arrive_to_execute into MUSTARRIVE,
+                 H_global_scheduling_invariant into INVARIANT,
+                 (*H_transitive into TRANS,
+                 H_unique_priorities into UNIQ,
+                 H_total into TOTAL,*)
+                 H_all_jobs_from_taskset into ALLJOBS,
+                 H_ts_is_a_set into SET.
+          clear ALLJOBS.
+
+          intros rt_bounds tsk R SOME IN j JOBj.
+          unfold R_list_edf, edf_rta_iteration in *.
+          assert (FIXED: forall tsk R,
+                           (tsk, R) \in rt_bounds ->
+                           R = task_cost tsk + response_time_bound tsk rt_bounds R).
+          {
+            admit.
+          }
+          generalize dependent j.
+          generalize dependent R.
+          generalize dependent tsk.
+
+          cut ((forall tsk R, (tsk, R) \in rt_bounds -> R = task_cost tsk + response_time_bound tsk rt_bounds R) -> (forall tsk R (j: JobIn arr_seq), (tsk, R) \in rt_bounds -> job_task j = tsk -> completed job_cost rate sched j (job_arrival j + R))).
+          {
+            by intro ASSUMP; ins; apply ASSUMP with (tsk := tsk).
+          }
+          {
+            ins.
+            admit.
+          }
+
+          (*
+          ins. 
+          unfold edf_schedulable, R_list_edf in *.
+
+
+          ins. 
+          induction ts as [| ts' tsk_i IH] using last_ind.
+          {
+            intros rt_bounds tsk R SOME IN.
+            by inversion SOME; subst; rewrite in_nil in IN.
+          }
+          {
+           intros rt_bounds tsk R SOME IN j JOBj.
+             destruct (lastP rt_bounds) as [| hp_bounds (tsk_lst, R_lst)];
+              first by rewrite in_nil in IN.
+            rewrite mem_rcons in_cons in IN; move: IN => /orP IN.
+            destruct IN as [LAST | BEGINNING]; last first.
+            {
+              apply IH with (rt_bounds := hp_bounds) (tsk := tsk); try (by ins).
+              by rewrite rcons_uniq in SET; move: SET => /andP [_ SET].
+              by ins; red; ins; apply TASKPARAMS; rewrite mem_rcons in_cons; apply/orP; right.
+              by ins; apply RESTR; rewrite mem_rcons in_cons; apply/orP; right.
+              by apply sorted_rcons_prefix in SORT.
+              {
+                intros tsk0 j0 t IN0 JOB0 BACK0.
+                exploit (INVARIANT tsk0 j0 t); try (by ins);
+                  [by rewrite mem_rcons in_cons; apply/orP; right | intro INV].
+                rewrite -cats1 count_cat /= in INV.
+                unfold is_interfering_task_fp in INV.
+                generalize SOME; apply R_list_rcons_task in SOME; subst tsk_i; intro SOME.
+                assert (HP: higher_eq_priority tsk_lst tsk0 = false).
+                {
+                  apply order_sorted_rcons with (x := tsk0) in SORT; [|by ins | by ins].
+                  apply negbTE; apply/negP; unfold not; intro BUG.
+                  exploit UNIQ; [by apply/andP; split; [by apply SORT | by ins] | intro EQ].
+                  by rewrite rcons_uniq -EQ IN0 in SET.
+                }              
+                by rewrite HP 2!andFb 2!addn0 in INV.
+              }
+              by apply R_list_rcons_prefix in SOME.
+            }
+            {
+              move: LAST => /eqP LAST.
+              inversion LAST as [[EQ1 EQ2]].
+              rewrite -> EQ1 in *; rewrite -> EQ2 in *; clear EQ1 EQ2 LAST.
+              generalize SOME; apply R_list_rcons_task in SOME; subst tsk_i; intro SOME.
+              generalize SOME; apply R_list_rcons_prefix in SOME; intro SOME'.
+              have BOUND := bertogna_cirinei_response_time_bound_fp.
+              unfold is_response_time_bound_of_task, job_has_completed_by in BOUND.
+              apply BOUND with (task_cost := task_cost) (task_period := task_period) (task_deadline := task_deadline) (job_deadline := job_deadline) (job_task := job_task) (tsk := tsk_lst)
+                               (ts := rcons ts' tsk_lst) (hp_bounds := hp_bounds)
+                               (higher_eq_priority := higher_eq_priority); clear BOUND; try (by ins).
+              by apply R_list_unzip1 with (R := R_lst).
+              {
+                intros hp_tsk R0 HP j0 JOB0.
+                apply IH with (rt_bounds := hp_bounds) (tsk := hp_tsk); try (by ins).
+                by rewrite rcons_uniq in SET; move: SET => /andP [_ SET].
+                by red; ins; apply TASKPARAMS; rewrite mem_rcons in_cons; apply/orP; right.
+                by ins; apply RESTR; rewrite mem_rcons in_cons; apply/orP; right.
+                by apply sorted_rcons_prefix in SORT.
+                {
+                  intros tsk0 j1 t IN0 JOB1 BACK0.
+                  exploit (INVARIANT tsk0 j1 t); try (by ins);
+                    [by rewrite mem_rcons in_cons; apply/orP; right | intro INV].
+                  rewrite -cats1 count_cat /= addn0 in INV.
+                  unfold is_interfering_task_fp in INV.
+                  assert (NOINTERF: higher_eq_priority tsk_lst tsk0 = false).
+                  {
+                    apply order_sorted_rcons with (x := tsk0) in SORT; [|by ins | by ins].
+                    apply negbTE; apply/negP; unfold not; intro BUG.
+                    exploit UNIQ; [by apply/andP; split; [by apply BUG | by ins] | intro EQ].
+                    by rewrite rcons_uniq EQ IN0 in SET.
+                  }
+                  by rewrite NOINTERF 2!andFb addn0 in INV.
+                }
+              }
+              by ins; apply R_list_ge_cost with (ts' := ts') (rt_bounds := hp_bounds).
+              by ins; apply R_list_le_deadline with (ts' := ts') (rt_bounds := hp_bounds).
+              {
+                ins; exploit (INVARIANT tsk_lst j0 t); try (by ins).
+                by rewrite mem_rcons in_cons; apply/orP; left.
+              }
+              {
+                rewrite [R_lst](R_list_rcons_response_time ts' hp_bounds tsk_lst); last by ins.
+                rewrite per_task_rta_fold.
+                apply per_task_rta_converges with (ts' := ts'); try (by ins).
+                {
+                  red; ins; apply TASKPARAMS.
+                  by rewrite mem_rcons in_cons; apply/orP; right.
+                }
+                apply R_list_le_deadline with (ts' := rcons ts' tsk_lst)
+                                            (rt_bounds := rcons hp_bounds (tsk_lst, R_lst));
+                  first by apply SOME'.
+                rewrite mem_rcons in_cons; apply/orP; left; apply/eqP.
+                f_equal; symmetry.
+                by apply R_list_rcons_response_time with (ts' := ts'). 
+              }
+            }
+          }*)
+        Qed.
+
+      End HelperLemma.
+      
+      (* If the schedulability test suceeds, ...*)
+      Hypothesis H_test_succeeds: edf_schedulable ts.
+      
+      (*..., then no task misses its deadline,... *)
+      Theorem taskset_schedulable_by_fp_rta :
+        forall tsk, tsk \in ts -> no_deadline_missed_by_task tsk.
+      Proof.
+        unfold no_deadline_missed_by_task, task_misses_no_deadline,
+               job_misses_no_deadline, completed,
+               edf_schedulable,
+               valid_sporadic_job in *.
+        rename H_valid_job_parameters into JOBPARAMS,
+               H_valid_task_parameters into TASKPARAMS,
+               H_restricted_deadlines into RESTR,
+               H_completed_jobs_dont_execute into COMP,
+               H_jobs_must_arrive_to_execute into MUSTARRIVE,
+               H_global_scheduling_invariant into INVARIANT,
+               (*H_sorted_ts into SORT,
+               H_transitive into TRANS,
+               H_unique_priorities into UNIQ,
+               H_total into TOTAL,*)
+               H_all_jobs_from_taskset into ALLJOBS,
+               H_test_succeeds into TEST.
+
+        admit.
+        
+        (*move => tsk INtsk j /eqP JOBtsk.
+        have RLIST := (R_list_has_response_time_bounds).
+        have NONEMPTY := (R_list_non_empty ts).
+        have DL := (R_list_le_deadline ts).
+
+        destruct (R_list ts) as [rt_bounds |]; last by ins.
+        exploit (NONEMPTY rt_bounds tsk); [by ins | intros [EX _]; specialize (EX INtsk); des].
+        exploit (RLIST rt_bounds tsk R); [by ins | by ins | by apply JOBtsk | intro COMPLETED].
+        exploit (DL rt_bounds tsk R); [by ins | by ins | clear DL; intro DL].
+        
+        rewrite eqn_leq; apply/andP; split; first by apply service_interval_le_cost.
+        apply leq_trans with (n := service rate sched j (job_arrival j + R)); last first.
+        {
+          unfold valid_sporadic_taskset, is_valid_sporadic_task in *.
+          apply service_monotonic; rewrite leq_add2l.
+          specialize (JOBPARAMS j); des; rewrite JOBPARAMS1.
+          by rewrite JOBtsk.
+        }
+        rewrite leq_eqVlt; apply/orP; left; rewrite eq_sym.
+        by apply COMPLETED.*)
+      Qed.
+
+      (* ..., and the schedulability test yields safe response-time
+         bounds for each task. *)
+      Theorem fp_schedulability_test_yields_response_time_bounds :
+        forall tsk,
+          tsk \in ts ->
+          exists R,
+            R <= task_deadline tsk /\
+            forall (j: JobIn arr_seq),
+              job_task j = tsk ->
+              completed job_cost rate sched j (job_arrival j + R).
+      Proof.
+        intros tsk IN.
+        admit.
+      (*unfold edf_schedulable in *.
+        have TASKS := R_list_non_empty ts.
+        have BOUNDS := (R_list_has_response_time_bounds).
+        have DL := (R_list_le_deadline ts).
+        destruct (R_list ts) as [rt_bounds |]; last by ins.
+        exploit (TASKS rt_bounds tsk); [by ins | clear TASKS; intro EX].
+        destruct EX as [EX _]; specialize (EX IN); des.
+        exists R; split.
+          by apply DL with (rt_bounds0 := rt_bounds).
+          by ins; apply (BOUNDS rt_bounds tsk). *)
+      Qed.
+
+      (* For completeness, since all jobs of the arrival sequence
+         are spawned by the task set, we conclude that no job misses
+         its deadline. *)
+      Theorem jobs_schedulable_by_fp_rta :
+        forall (j: JobIn arr_seq), no_deadline_missed_by_job j.
+      Proof.
+        intros j.
+        have SCHED := taskset_schedulable_by_fp_rta.
+        unfold no_deadline_missed_by_task, task_misses_no_deadline in *.
+        apply SCHED with (tsk := job_task j); last by rewrite eq_refl.
+        by apply H_all_jobs_from_taskset.
+      Qed.
+      
+    End Proof.
+
+  End Analysis.
+
+End ResponseTimeIterationEDF.
